lambda2Gmu/CanonicalForms.v
@@ -1,0 +1,41 @@
+Require Import Definitions.
+Require Import Infrastructure.
+Require Import TLC.LibTactics.
+Require Import TLC.LibEnv.
+Require Import TLC.LibLN.
+
+Lemma CanonicalFormTuple : forall Σ e T1 T2,
+    value e ->
+    {Σ, empty} ⊢ e ∈ T1 ** T2 ->
+    exists v1 v2, e = trm_tuple v1 v2.
+  introv.
+  intros Hv Ht.
+  inversion Hv; inversion Ht; subst; eauto; congruence.
+Qed.
+
+Lemma CanonicalFormAbs : forall Σ e T1 T2,
+    value e ->
+    {Σ, empty} ⊢ e ∈ T1 ==> T2 ->
+    exists v1, e = trm_abs T1 v1.
+  introv.
+  intros Hv Ht.
+  inversion Hv; inversion Ht; subst; eauto; congruence.
+Qed.
+
+Lemma CanonicalFormTAbs : forall Σ e T,
+    value e ->
+    {Σ, empty} ⊢ e ∈ typ_all T ->
+    exists v1, e = trm_tabs v1.
+  introv.
+  intros Hv Ht.
+  inversion Hv; inversion Ht; subst; eauto; congruence.
+Qed.
+
+Lemma CanonicalFormUnit : forall Σ e,
+    value e ->
+    {Σ, empty} ⊢ e ∈ typ_unit ->
+    e = trm_unit.
+  introv.
+  intros Hv Ht.
+  inversion Hv; inversion Ht; subst; eauto; congruence.
+Qed.
