lambda2Gmu/Progress.v
@@ -1,0 +1,103 @@
+Require Import Definitions.
+Require Import Infrastructure.
+Require Import CanonicalForms.
+Require Import TLC.LibTactics.
+Require Import TLC.LibEnv.
+Require Import TLC.LibLN.
+
+Ltac fs := exact \{}. (* There must be a better way *)
+Hint Resolve binds_empty_inv.
+
+Ltac empty_binding :=
+  match goal with
+  | H: binds ?x ?v empty |- _ => apply binds_empty_inv in H; contradiction
+  | _ => fail "no empty bindings found"
+  end.
+
+Lemma value_is_term : forall v,
+    value v -> term v.
+  induction 1; eauto.
+Qed.
+
+Lemma typed_is_term : forall Σ G T t,
+    {Σ, G} ⊢ t ∈ T ->
+    term t.
+  induction 1; subst; eauto.
+  - econstructor; eauto.
+    intros.
+    admit.
+  - econstructor; eauto.
+    inversion IHtyping; 
+      admit.
+Admitted.
+
+Ltac IHT e :=
+  match goal with
+  | Ht: {?Σ, ?E} ⊢ e ∈ ?T |- _ =>
+    match goal with
+    | IH: forall T, {Σ, E} ⊢ e ∈ T -> ?P |- _ =>
+      let H := fresh "IHt" in
+      assert P as H; eauto
+    end
+  end.
+
+Ltac copy H1 H2 :=
+  let Heq := fresh "Heq" in
+  remember H1 as H2 eqn:Heq; clear Heq.
+
+Hint Constructors value red.
+Theorem progress_thm : progress.
+  unfold progress.
+  intro.
+  induction e; introv; intros Htyp; inversion Htyp; subst.
+  - empty_binding.
+  - IHT e1. IHT e2.
+    destruct IHt as [IHv1 | IHev1].
+    + destruct IHt0 as [IHv2 | IHev2].
+      * left; eauto.
+      * inversion IHev2 as [e2' Hev2].
+        right; eauto.
+    + inversion IHev1; right; eauto.
+  - IHT e.
+    destruct IHt as [Hv | Hev].
+    copy Hv Hv'.
+    eapply CanonicalFormTuple in Hv; eauto.
+    inversion Hv as [v1 Hv2]; inversion Hv2 as [v2 Heq]; subst.
+    right; eauto.
+
+    inversion Hev as [e' ev]; eauto.
+  - IHT e.
+    destruct IHt as [Hv | Hev].
+    copy Hv Hv'.
+    eapply CanonicalFormTuple in Hv; eauto.
+    inversion Hv as [v1 Hv2]; inversion Hv2 as [v2 Heq]; subst.
+    right; eauto.
+
+    inversion Hev as [e' ev]; eauto.
+  - left; econstructor; econstructor; eauto.
+    intros; eapply typed_is_term; eauto. (* TODO ? *)
+  - IHT e1; IHT e2.
+    destruct IHt as [Hv1 | Hev1].
+    + destruct IHt0 as [Hv2 | Hev2].
+      * copy Hv1 Hv1'.
+        eapply CanonicalFormAbs in Hv1'; eauto.
+        inversion Hv1' as [v1 Heq]; subst.
+        right; eexists; econstructor; eauto.
+        eapply typed_is_term; eauto.
+      * right; inversion Hev2; eexists; eauto.
+    + right; inversion Hev1; eexists; eauto.
+  - left; econstructor; econstructor; eauto.
+    inversion Htyp; subst. (*TODO *) admit.
+  - IHT e.
+    destruct IHt as [Hv | Hev].
+    + right.
+      copy Hv Hv'.
+      eapply CanonicalFormTAbs in Hv'; eauto.
+      inversion Hv' as [v1 eq]; subst.
+      eexists. econstructor; eauto.
+      admit.
+      admit.
+    + admit.
+      Unshelve. fs.
+
+Qed.
